src/Prog.v
@@ -15,89 +15,52 @@ Set Implicit Arguments.
 (** * The programming language *)
 
 (** single program *)
-Polymorphic Inductive var_value : Type :=
-  | Any : forall (T : Type), T -> var_value.
-
 Inductive prog : Type -> Type :=
   | Ret T (v: T) : prog T
   | Read (a: addr) : prog valu
   | Write (a: addr) (v: valu) : prog unit
   | Sync : prog unit
   | Trim (a: addr) : prog unit
-  | VarAlloc (T : Type) (v : T) : prog nat
-  | VarDelete (i : nat) : prog unit
-  | VarGet (i : nat) (T : Type) : prog T
-  | VarSet (i : nat) (T : Type) (v : T) : prog unit
   | Hash (sz: nat) (buf: word sz) : prog (word hashlen)
   | Bind T T' (p1: prog T) (p2: T -> prog T') : prog T'.
 
 Arguments Ret {T} v.
-Arguments VarAlloc {T} v.
-Arguments VarGet i {T}.
-Arguments VarSet i {T} v.
-
-Definition varmem := @mem addr addr_eq_dec var_value.
 
 Inductive outcome (T : Type) :=
   | Failed
-  | Finished (m: rawdisk) (v: varmem) (hm: hashmap) (v: T)
+  | Finished (m: rawdisk) (hm: hashmap) (v: T)
   | Crashed (m: rawdisk) (hm: hashmap).
 
 Inductive step : forall T,
-    rawdisk -> varmem -> hashmap -> prog T ->
-    rawdisk -> varmem -> hashmap -> T -> Prop :=
-| StepRead : forall m a v x vm hm,
+    rawdisk -> hashmap -> prog T ->
+    rawdisk -> hashmap -> T -> Prop :=
+| StepRead : forall m a v x hm,
     m a = Some (v, x) ->
-    step m vm hm (Read a) m vm hm v
-| StepWrite : forall m a v v0 x vm hm,
+    step m hm (Read a) m hm v
+| StepWrite : forall m a v v0 x hm,
     m a = Some (v0, x) ->
-    step m vm hm (Write a v) (upd m a (v, v0 :: x)) vm hm tt
-| StepSync : forall m vm hm,
-    step m vm hm (Sync) (sync_mem m) vm hm tt
-| StepTrim : forall m a vs vs' vm hm,
+    step m hm (Write a v) (upd m a (v, v0 :: x)) hm tt
+| StepSync : forall m hm,
+    step m hm (Sync) (sync_mem m) hm tt
+| StepTrim : forall m a vs vs' hm,
     m a = Some vs ->
-    step m vm hm (Trim a) (upd m a vs') vm hm tt
-| StepHash : forall m sz (buf : word sz) h vm hm,
+    step m hm (Trim a) (upd m a vs') hm tt
+| StepHash : forall m sz (buf : word sz) h hm,
     hash_safe hm h buf ->
     hash_fwd buf = h ->
-    step m vm hm (Hash buf) m vm (upd_hashmap' hm h buf) h
-| StepVarAlloc : forall T d v vm i hm,
-    vm i = None ->
-    step d vm hm (@VarAlloc T v) d (insert vm i (@Any T v)) hm i
-| StepVarDelete : forall d v vm i hm,
-    vm i = Some v ->
-    step d vm hm (VarDelete i) d (delete vm i) hm tt
-| StepVarGet : forall T d v vm i hm,
-    vm i = Some (@Any T v) ->
-    step d vm hm (@VarGet i T) d vm hm v
-| StepVarSet : forall T d v0 v vm i hm,
-    vm i = Some v0 ->
-    step d vm hm (@VarSet i T v) d (upd vm i (@Any T v)) hm tt.
+    step m hm (Hash buf) m (upd_hashmap' hm h buf) h.
 
 Inductive fail_step : forall T,
-    rawdisk -> varmem -> prog T -> Prop :=
-| FailRead : forall m vm a,
+    rawdisk -> prog T -> Prop :=
+| FailRead : forall m a,
     m a = None ->
-    fail_step m vm (Read a)
-| FailWrite : forall m vm a v,
+    fail_step m (Read a)
+| FailWrite : forall m a v,
     m a = None ->
-    fail_step m vm (Write a v)
-| FailTrim : forall m vm a,
+    fail_step m (Write a v)
+| FailTrim : forall m a,
     m a = None ->
-    fail_step m vm (Trim a)
-| FailVarDelete : forall m vm i,
-    vm i = None ->
-    fail_step m vm (VarDelete i)
-| FailVarGetType : forall T T' m vm i (v : T'),
-    T <> T' ->
-    vm i = Some (Any v) ->
-    fail_step m vm (@VarGet i T)
-| FailVarGetNone : forall T m vm i,
-    vm i = None ->
-    fail_step m vm (@VarGet i T)
-| FailVarSetNone : forall T m vm i (v : T),
-    vm i = None ->
-    fail_step m vm (VarSet i v).
+    fail_step m (Trim a).
 
 Inductive crash_step : forall T, prog T -> Prop :=
 | CrashRead : forall a,
@@ -105,59 +68,59 @@ Inductive crash_step : forall T, prog T -> Prop :=
 | CrashWrite : forall a v,
     crash_step (Write a v).
 
-Inductive exec : forall T, rawdisk -> varmem -> hashmap -> prog T -> outcome T -> Prop :=
-| XRet : forall T m vm hm (v: T),
-    exec m vm hm (Ret v) (Finished m vm hm v)
-| XStep : forall T m vm hm (p: prog T) m' m'' vm' hm' v,
-    step m vm hm p m' vm' hm' v ->
+Inductive exec : forall T, rawdisk -> hashmap -> prog T -> outcome T -> Prop :=
+| XRet : forall T m hm (v: T),
+    exec m hm (Ret v) (Finished m hm v)
+| XStep : forall T m hm (p: prog T) m' m'' hm' v,
+    step m hm p m' hm' v ->
     possible_sync m' m'' ->
-    exec m vm hm p (Finished m'' vm' hm' v)
-| XBindFinish : forall m vm hm T (p1: prog T) m' vm' hm' (v: T)
+    exec m hm p (Finished m'' hm' v)
+| XBindFinish : forall m hm T (p1: prog T) m' hm' (v: T)
                   T' (p2: T -> prog T') out,
-    exec m vm hm p1 (Finished m' vm' hm' v) ->
-    exec m' vm' hm' (p2 v) out ->
-    exec m vm hm (Bind p1 p2) out
-| XBindFail : forall m vm hm T (p1: prog T)
+    exec m hm p1 (Finished m' hm' v) ->
+    exec m' hm' (p2 v) out ->
+    exec m hm (Bind p1 p2) out
+| XBindFail : forall m hm T (p1: prog T)
                 T' (p2: T -> prog T'),
-    exec m vm hm p1 (Failed T) ->
+    exec m hm p1 (Failed T) ->
     (* note p2 need not execute at all if p1 fails, a form of lazy
     evaluation *)
-    exec m vm hm (Bind p1 p2) (Failed T')
-| XBindCrash : forall m vm hm T (p1: prog T) m' hm'
+    exec m hm (Bind p1 p2) (Failed T')
+| XBindCrash : forall m hm T (p1: prog T) m' hm'
                  T' (p2: T -> prog T'),
-    exec m vm hm p1 (Crashed T m' hm') ->
-    exec m vm hm (Bind p1 p2) (Crashed T' m' hm')
-| XFail : forall m vm hm T (p: prog T),
-    fail_step m vm p ->
-    exec m vm hm p (Failed T)
-| XCrash : forall m vm hm T (p: prog T),
+    exec m hm p1 (Crashed T m' hm') ->
+    exec m hm (Bind p1 p2) (Crashed T' m' hm')
+| XFail : forall m hm T (p: prog T),
+    fail_step m p ->
+    exec m hm p (Failed T)
+| XCrash : forall m hm T (p: prog T),
     crash_step p ->
-    exec m vm hm p (Crashed T m hm).
+    exec m hm p (Crashed T m hm).
 
 (** program with recovery *)
 Inductive recover_outcome (TF TR: Type) :=
   | RFailed
-  | RFinished (m: rawdisk) (vm: varmem) (hm: hashmap) (v: TF)
-  | RRecovered (m: rawdisk) (vm: varmem) (hm: hashmap) (v: TR).
+  | RFinished (m: rawdisk) (hm: hashmap) (v: TF)
+  | RRecovered (m: rawdisk) (hm: hashmap) (v: TR).
 
 Inductive exec_recover (TF TR: Type)
-    : rawdisk -> varmem -> hashmap -> prog TF -> prog TR -> recover_outcome TF TR -> Prop :=
-  | XRFail : forall m vm hm p1 p2, exec m vm hm p1 (Failed TF)
-    -> exec_recover m vm hm p1 p2 (RFailed TF TR)
-  | XRFinished : forall m vm hm p1 p2 m' vm' hm' (v: TF), exec m vm hm p1 (Finished m' vm' hm' v)
-    -> exec_recover m vm hm p1 p2 (RFinished TR m' vm' hm' v)
-  | XRCrashedFailed : forall m vm hm p1 p2 m' hm' m'r, exec m vm hm p1 (Crashed TF m' hm')
+    : rawdisk -> hashmap -> prog TF -> prog TR -> recover_outcome TF TR -> Prop :=
+  | XRFail : forall m hm p1 p2, exec m hm p1 (Failed TF)
+    -> exec_recover m hm p1 p2 (RFailed TF TR)
+  | XRFinished : forall m hm p1 p2 m' hm' (v: TF), exec m hm p1 (Finished m' hm' v)
+    -> exec_recover m hm p1 p2 (RFinished TR m' hm' v)
+  | XRCrashedFailed : forall m hm p1 p2 m' hm' m'r, exec m hm p1 (Crashed TF m' hm')
     -> possible_crash m' m'r
-    -> @exec_recover TR TR m'r empty_mem hm' p2 p2 (RFailed TR TR)
-    -> exec_recover m vm hm p1 p2 (RFailed TF TR)
-  | XRCrashedFinished : forall m vm hm p1 p2 m' hm' m'r m'' vm'' hm'' (v: TR), exec m vm hm p1 (Crashed TF m' hm')
+    -> @exec_recover TR TR m'r hm' p2 p2 (RFailed TR TR)
+    -> exec_recover m hm p1 p2 (RFailed TF TR)
+  | XRCrashedFinished : forall m hm p1 p2 m' hm' m'r m'' hm'' (v: TR), exec m hm p1 (Crashed TF m' hm')
     -> possible_crash m' m'r
-    -> @exec_recover TR TR m'r empty_mem hm' p2 p2 (RFinished TR m'' vm'' hm'' v)
-    -> exec_recover m vm hm p1 p2 (RRecovered TF m'' vm'' hm'' v)
-  | XRCrashedRecovered : forall m vm hm p1 p2 m' hm' m'r m'' vm'' hm'' (v: TR), exec m vm hm p1 (Crashed TF m' hm')
+    -> @exec_recover TR TR m'r hm' p2 p2 (RFinished TR m'' hm'' v)
+    -> exec_recover m hm p1 p2 (RRecovered TF m'' hm'' v)
+  | XRCrashedRecovered : forall m hm p1 p2 m' hm' m'r m'' hm'' (v: TR), exec m hm p1 (Crashed TF m' hm')
     -> possible_crash m' m'r
-    -> @exec_recover TR TR m'r empty_mem hm' p2 p2 (RRecovered TR m'' vm'' hm'' v)
-    -> exec_recover m vm hm p1 p2 (RRecovered TF m'' vm'' hm'' v).
+    -> @exec_recover TR TR m'r hm' p2 p2 (RRecovered TR m'' hm'' v)
+    -> exec_recover m hm p1 p2 (RRecovered TF m'' hm'' v).
 
 Hint Constructors exec.
 Hint Constructors step.
